src/fourbitcounter_OK.v
@@ -1,0 +1,20 @@
+Require Import Bool String List.
+Require Import Lib.CommonTactics Lib.ilist Lib.Word.
+Require Import Lib.Struct Lib.FMap Lib.StringEq Lib.Indexer.
+Require Import Kami.Syntax Kami.Semantics Kami.RefinementFacts Kami.Renaming Kami.Wf.
+Require Import Kami.Renaming Kami.Inline Kami.InlineFacts.
+Require Import Kami.Decomposition Kami.Notations Kami.Tactics.
+Require Import Kami.PrimFifo.
+Require Import Init.Nat.
+
+Require Import fourbitcount2.
+
+Set Implicit Arguments.
+
+Theorem fourbitcounter_OK :
+   fourbitcount2.spec.spec "top" <<== fourbitcount2.module'mkTb.mkTb "top".
+
+Proof.
+admit. (* fixme: proof goes here *)
+
+Admitted.
